chore: Prove correctness of new k-induction (#1357)

SSA/Experimental/Bits/Fast/ReflectVerif.lean
@@ -6,6 +6,9 @@ into lean bitvectors.
 We use `bv_circuit_nnf` to convert the expression into negation normal form.
 
 Authors: Siddharth Bhat
+
+https://raw.githubusercontent.com/opencompl/lean-mlir/3e0ff379b5e92427747f8dc84c6f77609bda7e67/SSA/Experimental/Bits/Fast/ReflectVerif.lean
+
 -/
 import Mathlib.Data.Bool.Basic
 import Mathlib.Data.Fin.Basic
@@ -421,6 +424,12 @@ def castLe (i : Inputs ι n) (hn : n ≤ m) : Inputs ι m where
   input := i.input
 
 @[simp]
+theorem castLe_mk_eq_mk {α : Type _} {n m : Nat} (i : Fin n) (h : n ≤ m) (x : α) :
+    (Inputs.mk i x).castLe h = Inputs.mk (i.castLE (by omega)) x := by
+  simp [Inputs.castLe, Inputs.mk]
+  rfl
+
+@[simp]
 theorem castLe_eq_self {α : Type _} {n : Nat} (i : Inputs α n) (h : n ≤ n) :
     i.castLe h = i := by
   simp [Inputs.castLe]
@@ -501,6 +510,16 @@ def Vars.state0 (s : σ) {n : Nat} : Vars σ ι n :=
 def Vars.stateN (s : σ) (i : Nat) {n : Nat} (hin : i ≤ n := by omega) : Vars σ ι n :=
   .state (Inputs.mk ⟨i, by omega⟩ s)
 
+@[simp]
+theorem state0_eq_stateN_zero {σ : Type} {ι : Type} {n : Nat} (s : σ) :
+    (Vars.state0 s : Vars σ ι n) = Vars.stateN s 0 := by
+  simp [Vars.state0, Vars.stateN]
+
+theorem stateN_zero_eq_state0 {σ : Type} {ι : Type} {n : Nat} (s : σ) :
+    Vars.stateN s 0 = (Vars.state0 s : Vars σ ι n) := by
+  simp [Vars.state0, Vars.stateN]
+
+
 def Vars.inputN (inp : ι) (k : Nat) {n : Nat} (hkn : k < n := by omega) : Vars σ ι n :=
   .inputs (Inputs.mk ⟨k, by omega⟩ inp)
 
@@ -554,12 +573,38 @@ def Vars.castShift {n m : Nat} (v : Vars σ ι n) (hnm : n ≤ m) : Vars σ ι m
 
 /-- casting to the same width equals vars-/
 @[simp]
-theorem Vars.castLe_eq_self {α : Type _} {n : Nat} (v : Vars α σ n) (h : n ≤ n) :
+theorem Vars.castLe_eq_self {n : Nat} (v : Vars σ ι n) (h : n ≤ n) :
     v.castLe h = v := by
   rcases v with x | i
   · simp [Vars.castLe]
   · simp [Vars.castLe]
   · simp [Vars.castLe]
+
+@[simp]
+theorem Vars.castLe_outputs_mk_eq_outputs {n i m : Nat} (hi : i < n) (hnm : n ≤ m) :
+  ((Vars.outputs ⟨i, hi⟩ : Vars σ ι n).castLe (by omega) : Vars σ ι m) =
+     Vars.outputs ⟨i, by omega⟩ := by
+  simp [Vars.castLe, Vars.outputs]
+
+@[simp]
+theorem Vars.castLe_stateN_eq_stateN  {n i m : Nat} (hi : i ≤ n) (hnm : n ≤ m) :
+  (Vars.stateN s i : Vars σ ι n).castLe hnm =
+  Vars.stateN s i (hin := by omega) := by
+  rfl
+
+@[simp]
+theorem Vars.castLe_state_Inputs_mk_eq_state_castLe_Inputs_mk {n m : Nat}
+    (hnm : n ≤ m) {s : σ} {i : Fin (n + 1)} :
+    (Vars.state (Inputs.mk i s) : Vars σ ι n).castLe hnm =
+    (Vars.state (Inputs.mk (i.castLE (by omega)) s) : Vars σ ι m) := by
+  simp [Vars.castLe, Vars.state]
+
+
+@[simp]
+theorem Vars.castLe_inputs_eq_inputs {n i m : Nat} (hi : i < n) (hnm : n ≤ m) :
+  (Vars.inputN inp i hi : Vars σ ι n).castLe hnm =
+  Vars.inputN inp i (by omega) := by
+  rfl
 
 /-- casting to the same width equals vars-/
 @[simp]
@@ -573,24 +618,107 @@ theorem Vars.castLe_castLe_eq_castLe_self {α : Type _} {p q r : Nat}
 
 
 /-- Relate boolean and bitstream environments. -/
-structure EnvOutRelated {arity : Type _} {α : Type _}
+structure EnvSimEnvBitstream {arity : Type _} {α : Type _}
     (envBool : Vars α arity n → Bool)
     (envBitstream : arity → BitStream) where
   envBool_inputs_mk_eq_envBitStream : ∀ (x : arity) (i : Nat) (hi: i < n),
     envBool (Vars.inputs (Inputs.mk ⟨i, by omega⟩ x)) = envBitstream x i
 
 
-theorem EnvOutRelated.envBool_inputs_mk_castShift_eq_envBitStream
+theorem EnvSimEnvBitstream.envBool_inputs_mk_castShift_eq_envBitStream
    (envBool : Vars α arity m → Bool)
    (envBitstream : arity → BitStream)
-   (hEnvBitstream : EnvOutRelated envBool envBitstream)
+   (hEnvBitstream : EnvSimEnvBitstream envBool envBitstream)
    (hnm : n ≤ m) (x : arity) (i : Nat) (hi : i < n) :
    (envBool ((Vars.inputs (Inputs.mk ⟨i, by omega⟩ x : Inputs _ n) :  Vars _ _ n).castShift hnm))=
    envBitstream x (m - 1 - i) := by
   rw [← hEnvBitstream.envBool_inputs_mk_eq_envBitStream]
   rfl
 
-attribute [simp] EnvOutRelated.envBool_inputs_mk_eq_envBitStream
+attribute [simp] EnvSimEnvBitstream.envBool_inputs_mk_eq_envBitStream
+
+/-- Environment with chosen state variables of the FSM. -/
+def envBool_of_envBitstream_of_state (p : FSM arity)
+   (envBitstream : arity → BitStream)
+   (s0 : p.α → Bool)
+   (n : Nat) : Vars p.α arity (n + 1) → Bool :=
+  fun x =>
+    match x with
+    | .state ss =>
+      p.carryWith s0 envBitstream ss.ix ss.input
+    | .inputs (.mk a i) => envBitstream i a
+    | .outputs o =>
+      p.evalWith s0 envBitstream o
+
+
+/-- Environment with chosen state variables of the FSM. -/
+def envBoolStart_of_envBitstream (p : FSM arity)
+   (envBitstream : arity → BitStream)
+   (n : Nat) : Vars p.α arity (n + 1) → Bool :=
+  envBool_of_envBitstream_of_state p envBitstream p.initCarry n
+
+/-
+@[simp]
+theorem envBool_of_envBitstream_of_state_eq₁ {arity : Type _} {α : Type _}
+    (envBitstream : arity → BitStream) (s0 : α → Bool) (n : Nat)
+    (s : α) :
+    envBool_of_envBitstream_of_state envBitstream s0 n (.state s) = s0 s := rfl
+
+@[simp]
+theorem envBool_of_envBitstream_of_state_eq₂ {arity : Type _} {α : Type _}
+    (envBitstream : arity → BitStream) (state : α → Bool) (n : Nat)
+    (i : Inputs arity (n + 1)) :
+    envBool_of_envBitstream_of_state envBitstream state n (.inputs i) =
+    envBitstream i.input i.ix := rfl
+
+def Bitstream_of_envBool
+  (envBool : Vars α arity n → Bool) :
+  (arity → BitStream) :=
+  fun a =>
+    fun k =>
+      if hk : k < n
+      then envBool (.inputs (Inputs.mk ⟨k, by omega⟩ a))
+      else false
+
+/-- make the init carry of the FSM from the envBool. -/
+def initCarry_of_envBool {p : FSM α}
+  (envBool : Vars p.α arity n → Bool) :
+  p.α → Bool := fun a => envBool (.state a)
+
+@[simp]
+theorem EnvOutRelated_envBoolEmpty_of_envBitStream_of_self {arity : Type _}
+    (envBitstream : arity → BitStream) :
+    EnvOutRelated (envBoolEmpty_of_envBitstream envBitstream n) envBitstream := by
+  constructor
+  intros x i hi
+  rw [envBoolEmpty_of_envBitstream]
+
+@[simp]
+theorem EnvOutRelated_envBoolStart_of_envBitStream_of_self {arity : Type _} {α : Type _}
+    (p : FSM α) (envBitstream : arity → BitStream) :
+    EnvOutRelated (envBoolStart_of_envBitstream p envBitstream n) envBitstream := by
+  constructor
+  intros x i hi
+  rw [envBoolStart_of_envBitstream]
+
+@[simp]
+theorem EnvOutRelated_envBoolStart_ofenvBitstream_of_state_of_self
+    {arity : Type _} {α : Type _}
+    (envBitstream : arity → BitStream) (state : α → Bool) :
+    EnvOutRelated (envBool_of_envBitstream_of_state envBitstream state n) envBitstream := by
+  constructor
+  intros x i hi
+  rw [envBool_of_envBitstream_of_state]
+
+@[simp]
+theorem EnvOutRelated_self_Bitstream_of_envBool
+    (envBool : Vars α arity n → Bool) :
+    EnvOutRelated envBool (Bitstream_of_envBool envBool) := by
+  constructor
+  intros x i hi
+  simp [Bitstream_of_envBool, hi]
+-/
+
 
 /-- Take the 'or' of many circuits.-/
 def Circuit.bigOr {α : Type _}
@@ -712,7 +840,8 @@ deriving Repr, Inhabited, DecidableEq, Hashable
 
 
 /--
-Make the funtion that for a given state 's', computes `carry(states[n][s], inputs[n])`.
+Make the funtion that for a given state 's', computes
+`states[n+1][s] = carry[s](states[n][:], inputs[n])`.
 --/
 def mkCarryAssignCircuitNAux {arity : Type _}
   [DecidableEq arity]
@@ -725,8 +854,48 @@ def mkCarryAssignCircuitNAux {arity : Type _}
         | .inr i => Vars.inputN i n
 
 /--
+The MkcarryAssign circuit is false iff
+p.nextBitCirc evaluates to false on the given environment.
+-/
+theorem mkCarryAssignCircuitNAux_eval_eq_ {arity : Type _}
+    [DecidableEq arity]
+    [Fintype arity]
+    [Hashable arity]
+    (p : FSM arity) (s : p.α) (n : Nat)
+    {env : Vars p.α arity (n + 1) → Bool}
+    {env' : p.α ⊕ arity → Bool}
+    (hEnvState : ∀ (s : p.α), env (Vars.stateN s n) = env' (Sum.inl s))
+    (hEnvInput : ∀ (i : arity), env (Vars.inputN i n) = env' (Sum.inr i)) :
+    ((mkCarryAssignCircuitNAux p s n).eval env) = ((p.nextBitCirc (some s)).eval env') := by
+  rw [mkCarryAssignCircuitNAux]
+  rw [Circuit.eval_map]
+  congr
+  ext x
+  rcases x with x | x
+  · simp [hEnvState]
+  · simp [hEnvInput]
+/--
+The MkcarryAssign circuit is false iff
+p.nextBitCirc evaluates to false on the given environment.
+-/
+@[simp]
+theorem mkCarryAssignCircuitNAux_eval_eq {arity : Type _}
+    [DecidableEq arity]
+    [Fintype arity]
+    [Hashable arity]
+    (p : FSM arity) (s : p.α) (n : Nat)
+    {env : Vars p.α arity (n + 1) → Bool} :
+    ((mkCarryAssignCircuitNAux p s n).eval env) = ((p.nextBitCirc (some s)).eval
+      (fun x => match x with | .inl x => env (Vars.stateN x n) | .inr x => env (Vars.inputN x n))) := by
+  rw [mkCarryAssignCircuitNAux]
+  rw [Circuit.eval_map]
+  congr
+  ext x
+  rcases x with x | x <;> simp
+
+/--
 Make the circuit that assigns the carry state:
-  `states[n+1][:] = carry(states[n][:], inputs[n][:])`.
+  `states[n+1][:] = carry[:](states[n][:], inputs[n][:])`.
 -/
 def mkCarryAssignCircuitN {arity : Type _}
   [DecidableEq arity]
@@ -740,6 +909,25 @@ def mkCarryAssignCircuitN {arity : Type _}
       (mkCarryAssignCircuitNAux p s n)
       (Circuit.var true <| Vars.stateN s (n + 1))
   Circuit.bigOr carrys
+
+@[simp]
+theorem eval_mkCarryAssignCircuitN_eq_false_iff {arity : Type _}
+  [DecidableEq arity]
+  [Fintype arity]
+  [Hashable arity]
+  (p : FSM arity) (n : Nat)
+  {env : Vars p.α arity (n + 1) → Bool} :
+  ((mkCarryAssignCircuitN p n).eval env = false) ↔
+    (∀ (s : p.α), env (Vars.stateN s (n + 1)) = (mkCarryAssignCircuitNAux p s n).eval env) := by
+  rw [mkCarryAssignCircuitN]
+  simp
+  constructor
+  · intros h s
+    specialize h s
+    rw [← h]
+  · intros h s
+    specialize h s
+    rw [← h]
 
 /--
 Make the circuit that assigns `states[i][:] = carry(states[i-1][:], inputs[i-1][:])`
@@ -756,6 +944,33 @@ def mkCarryAssignCircuitLeN {arity : Type _}
       mkCarryAssignCircuitN p i |>.map (fun v => v.castLe (by simp at hi; omega))
     Circuit.bigOr circs
 
+@[simp]
+theorem mkCarryAssignCircuitLeN_eq_false_iff {arity : Type _}
+  [DecidableEq arity] [Fintype arity] [Hashable arity] (p : FSM arity) (n : Nat)
+  (env : Vars p.α arity (n + 1) → Bool) :
+  ((mkCarryAssignCircuitLeN p n).eval env = false) ↔
+  (∀ (s : p.α) (i : Nat), (hi : i < n + 1) →
+    env (Vars.stateN s (i + 1)) =
+     ((mkCarryAssignCircuitNAux p s i).map (fun v => v.castLe (by omega))).eval env) := by
+  rw [mkCarryAssignCircuitLeN]
+  simp only [Circuit.eval_bigOr_eq_false_iff, List.mem_map, List.mem_attach, true_and,
+    Subtype.exists, List.mem_range, forall_exists_index]
+  constructor
+  · intros h s i hi
+    specialize h ?c i (by omega) rfl
+    simp only [Circuit.eval_map, eval_mkCarryAssignCircuitN_eq_false_iff,
+      mkCarryAssignCircuitNAux_eval_eq] at h
+    simp only [Circuit.eval_map, mkCarryAssignCircuitNAux_eval_eq]
+    apply h
+  · intros h c i hi hc
+    subst hc
+    simp only [Circuit.eval_map, eval_mkCarryAssignCircuitN_eq_false_iff,
+      mkCarryAssignCircuitNAux_eval_eq]
+    intros s
+    specialize h s i hi
+    simp only [Circuit.eval_map, mkCarryAssignCircuitNAux_eval_eq] at h
+    apply h
+
 /--
 Make the circuit that assigns `states[0][s] = initCarry[s]`.
 -/
@@ -769,6 +984,20 @@ def mkInitCarryAssignCircuitAux {arity : Type _}
       (Circuit.ofBool (p.initCarry s))
       (Circuit.var true <| Vars.stateN s 0)
 
+theorem mkInitCarryAssignCircuitAux_eq_false_iff {arity : Type _}
+  [DecidableEq arity]
+  [Fintype arity]
+  [Hashable arity]
+  (p : FSM arity) (s : p.α)
+  {env : Vars p.α arity 0 → Bool}:
+  ((mkInitCarryAssignCircuitAux p s).eval env = false) ↔
+  (p.initCarry s = env (Vars.stateN s 0)) := by
+  rw [mkInitCarryAssignCircuitAux]
+  simp
+  rcases hx : p.initCarry s
+  · simp
+  · simp
+
 /--
 Make the circuit that assigns `states[0][:] = initCarry[:]`.
 -/
@@ -780,6 +1009,17 @@ def mkInitCarryAssignCircuit {arity : Type _}
   Circuit (Vars p.α arity 0) :=
     let carrys := FinEnum.toList p.α |>.map (mkInitCarryAssignCircuitAux p)
     Circuit.bigOr carrys
+
+theorem eval_mkInitCarryAssignCircuit_eq_false_iff {arity : Type _}
+  [DecidableEq arity]
+  [Fintype arity]
+  [Hashable arity]
+  (p : FSM arity)
+  {env : Vars p.α arity 0 → Bool} :
+  (mkInitCarryAssignCircuit p).eval env = false ↔
+  (∀ (s : p.α), p.initCarry s = env (Vars.state0 s)) := by
+  rw [mkInitCarryAssignCircuit]
+  simp [mkInitCarryAssignCircuitAux_eq_false_iff]
 
 /--
 Make a circuit that computes `out(states[n][:], inputs[n][:])`.
@@ -794,6 +1034,23 @@ def mkOutputAssignCircuitNAux {arity : Type _}
         | .inl s' => Vars.stateN s' n
         | .inr i => Vars.inputN i n
 
+@[simp]
+theorem eval_mkOutputAssignCircuitNAux_eq {arity : Type _}
+  [DecidableEq arity]
+  [Fintype arity]
+  [Hashable arity]
+  (p : FSM arity) (n : Nat) (env : Vars p.α arity (n + 1) → Bool) :
+  (mkOutputAssignCircuitNAux p n).eval env =
+    (p.nextBitCirc none).eval
+      (fun x => match x with
+        | .inl s => env (Vars.stateN s n)
+        | .inr i => env (Vars.inputN i n)) := by
+  rw [mkOutputAssignCircuitNAux]
+  simp [Circuit.eval_map]
+  congr
+  ext x
+  rcases x with x | x <;> simp
+
 /-- Make a circuit that assigns
 `out[n] = out(states[n][:], inputs[n][:])`.
 -/
@@ -806,6 +1063,23 @@ def mkOutputAssignCircuitN {arity : Type _}
     Circuit.xor
       (mkOutputAssignCircuitNAux p n)
       (Circuit.var true <| Vars.outputs ⟨n, by omega⟩)
+
+@[simp]
+theorem eval_mkOutputAssignCircuitN_eq_false_iff {arity : Type _}
+  [DecidableEq arity]
+  [Fintype arity]
+  [Hashable arity]
+  (p : FSM arity) (n : Nat)
+  {env : Vars p.α arity (n + 1) → Bool}
+  :
+  ((mkOutputAssignCircuitN p n).eval env = false) ↔
+    (p.nextBitCirc none).eval
+      (fun x => match x with
+        | .inl s => env (Vars.stateN s n)
+        | .inr i => env (Vars.inputN i n)) =
+    env (Vars.outputs ⟨n, by omega⟩) := by
+  rw [mkOutputAssignCircuitN]
+  simp [Circuit.eval_map, eval_mkOutputAssignCircuitNAux_eq]
 
 
 def mkOutputAssignCircuitLeN {arity : Type _}
@@ -820,9 +1094,36 @@ def mkOutputAssignCircuitLeN {arity : Type _}
     Circuit.bigOr circs
 
 
+theorem mkOutputAssignCircuitLeN_eq_false_iff {arity : Type _}
+  [DecidableEq arity] [Fintype arity] [Hashable arity] (p : FSM arity) (n : Nat)
+  (env : Vars p.α arity (n + 1) → Bool) :
+  ((mkOutputAssignCircuitLeN p n).eval env = false) ↔
+  (∀ (i : Nat) (hi : i < n + 1),
+    (p.nextBitCirc none).eval
+      (fun x => match x with
+        | .inl s => env (Vars.stateN s i)
+        | .inr j => env (Vars.inputN j i)) =
+    env (Vars.outputs ⟨i, by omega⟩)) := by
+  rw [mkOutputAssignCircuitLeN]
+  simp only [Circuit.eval_bigOr_eq_false_iff, List.mem_map, List.mem_attach, true_and,
+    Subtype.exists, List.mem_range, forall_exists_index]
+  constructor
+  · intros h i hi
+    specialize h ?c i (by omega) rfl
+    simp only [Circuit.eval_map, eval_mkOutputAssignCircuitN_eq_false_iff] at h
+    apply h
+  · intros h c i hi hc
+    subst hc
+    simp only [Circuit.eval_map, eval_mkOutputAssignCircuitN_eq_false_iff]
+    simp only [Circuit.eval_map, eval_mkOutputAssignCircuitNAux_eq] at h
+    specialize h i hi
+    simp only [Vars.castLe_outputs_mk_eq_outputs]
+    rw [← h]
+    congr
 /--
 Make a circuit that checks `out[n] = fals`.
 -/
+@[simp]
 def mkOutEqZeroCircuitN {arity : Type _}
   [DecidableEq arity]
   [Fintype arity]
@@ -835,6 +1136,17 @@ def mkOutEqZeroCircuitN {arity : Type _}
       (Circuit.ofBool false)
       (Circuit.var true <| Vars.outputs ⟨n, by omega⟩)
 
+@[simp]
+theorem mkOutEqZeroCircuitN_eval_eq_false_iff {arity : Type _}
+  [DecidableEq arity]
+  [Fintype arity]
+  [Hashable arity]
+  (p : FSM arity) (n : Nat)
+  {env : Vars p.α arity (n + 1) → Bool} :
+  ((mkOutEqZeroCircuitN p n).eval env = false) ↔
+    env (Vars.outputs ⟨n, by omega⟩) = false := by
+  rw [mkOutEqZeroCircuitN]
+  simp
 
 /--
 Make a circuit that checks `out[n] = fals` for all `i ≤ n`
@@ -849,6 +1161,32 @@ def mkOutEqZeroCircuitLeN {arity : Type _}
     let circs := ixs.map fun ⟨i, hi⟩ =>
       mkOutEqZeroCircuitN p i |>.map (fun v => v.castLe (by simp at hi; omega))
     Circuit.bigOr circs
+
+theorem mkOutEqZeroCircuitLeN_eval_eq_false_iff {arity : Type _}
+  [DecidableEq arity] [Fintype arity] [Hashable arity] (p : FSM arity) (n : Nat)
+  (env : Vars p.α arity (n + 1) → Bool) :
+  ((mkOutEqZeroCircuitLeN p n).eval env = false) ↔
+  (∀ (i : Nat) (hi : i < n + 1),
+    env (Vars.outputs ⟨i, by omega⟩) = false) := by
+  rw [mkOutEqZeroCircuitLeN]
+  simp only [Circuit.eval_bigOr_eq_false_iff, List.mem_map, List.mem_attach, true_and,
+    Subtype.exists, List.mem_range, forall_exists_index]
+  constructor
+  · intros h i hi
+    specialize h ?c i (by omega) rfl
+    simp only [Circuit.eval_map, mkOutEqZeroCircuitN_eval_eq_false_iff] at h
+    apply h
+  · intros h c i hi hc
+    subst hc
+    simp only [Circuit.eval_map, mkOutEqZeroCircuitN_eval_eq_false_iff]
+    apply h i hi
+
+theorem mkOutEqZeroCircuitLeN_eval_eq_false_iff₂ {arity : Type _}
+  [DecidableEq arity] [Fintype arity] [Hashable arity] (p : FSM arity) (n : Nat) :
+  (∀ (env : Vars p.α arity (n + 1) → Bool), (mkOutEqZeroCircuitLeN p n).eval env = false) ↔
+  (∀ (env : Vars p.α arity (n + 1) → Bool) (i : Nat), (hi : i < n + 1) → env (Vars.outputs ⟨i, by omega⟩) = false) := by
+  simp [mkOutEqZeroCircuitLeN_eval_eq_false_iff]
+
 
 def mkUnsatImpliesCircuit (lhs rhs : Circuit α) : Circuit α :=
   -- truth table of this circuit:
@@ -905,14 +1243,19 @@ def mkLowerTriangularPairs (n : Nat) : List (Nat × Nat) :=
     let ys := List.range i.val |>.attach
     ys.map fun j => (j.val, i.val)
 
-
 @[simp]
-theorem mem_mkLowerTriangularPairs {n : Nat} (i j : Nat) :
-  (i, j) ∈ mkLowerTriangularPairs n ↔
+theorem mem_mkLowerTriangularPairs {n : Nat} {i j : Nat} :
+  ((i, j) ∈ mkLowerTriangularPairs n) ↔
   (i < j ∧ j ≤ n) := by
   simp [mkLowerTriangularPairs]
   omega
 
+@[simp]
+theorem mem_mkLowerTriangularPairs₂  {n : Nat} {ij :  Nat × Nat} :
+  (ij ∈ mkLowerTriangularPairs n) ↔
+  (ij.1 < ij.2 ∧ ij.2 ≤ n) := by
+  obtain ⟨i, j⟩ := ij
+  simp
 
 /--
 make the circuit that says that the state at index 'n' is disequal from all states [0..n)
@@ -928,6 +1271,23 @@ def mkStateUniqueCircuitN {arity : Type _}
     (mkStateNeqCircuit p si sn)
   Circuit.bigOr circs
 
+theorem mkStateUniqueCircuitN_eq_false_iff {arity : Type _}
+  [DecidableEq arity] [Fintype arity] [Hashable arity]
+  (p : FSM arity) (n : Nat)
+  {env : Vars p.α arity n → Bool} :
+  ((mkStateUniqueCircuitN p n).eval env = false) ↔
+  (∀ (i : Nat) (hi : i < n), ∃ (s : p.α), env (Vars.stateN s i) ≠ env (Vars.stateN s n)) := by
+  rw [mkStateUniqueCircuitN]
+  simp only [Circuit.eval_bigOr_eq_false_iff, List.mem_map, List.mem_attach, true_and,
+    Subtype.exists, List.mem_range, forall_exists_index]
+  constructor
+  · intros h i hi
+    specialize h ?c i hi rfl
+    simpa using h
+  · intros h c i hi hc
+    subst hc
+    specialize h i hi
+    simpa using h
 /--
 make the circuit that witnesses that the states are unique from [0..n]
 -/
@@ -942,7 +1302,27 @@ def mkAllPairsUniqueStatesCircuit {arity : Type _}
       Circuit.var true (Vars.stateN s j (by simp at hij; omega))
     (mkStateNeqCircuit p si sj)
 
-
+theorem mkAllPairsUniqueStatesCircuit_eq_false_iff {arity : Type _}
+  [DecidableEq arity] [Fintype arity] [Hashable arity]
+  (p : FSM arity) (n : Nat)
+  {env : Vars p.α arity n → Bool} :
+  ((mkAllPairsUniqueStatesCircuit p n).eval env = false) ↔
+  (∀ (i j : Nat) (hij : i < j ∧ j ≤ n), ∃ (s : p.α), env (Vars.stateN s i) ≠ env (Vars.stateN s j)) := by
+  rw [mkAllPairsUniqueStatesCircuit]
+  simp only [Circuit.eval_bigOr_eq_false_iff, List.mem_map, List.mem_attach, true_and,
+    Subtype.exists, List.mem_range, forall_exists_index]
+  constructor
+  · intros h i j hij
+    simp only [Prod.forall, mem_mkLowerTriangularPairs] at h
+    specialize h ?c i j hij rfl
+    simpa using h
+  · intros h c ij hij hc
+    subst hc
+    simp only [mkStateNeqCircuit_eq_false_iff₂, Circuit.eval, ↓reduceIte, ne_eq]
+    obtain ⟨i, j⟩ := ij
+    simp only [mem_mkLowerTriangularPairs₂] at hij
+    simp only [ne_eq] at ⊢ h
+    apply h i j hij
 
 /-- structure for incrementally building the k-induction circuits. -/
 structure KInductionCircuits {arity : Type _}
@@ -954,12 +1334,46 @@ structure KInductionCircuits {arity : Type _}
   -- | Circuit that sets out[i] = out(states[i], inputs[i]) upto 'n'.
   cOutAssignCirc : Circuit (Vars fsm.α arity (n + 2))
   -- | Circuit that says that states s0..sn are disequal
-  cStatesUniqueCirc : Circuit (Vars fsm.α arity (n + 1))
+  cStatesUniqueCirc : Circuit (Vars fsm.α arity n)
+
+structure KInductionCircuits.IsLawful {arity : Type _}
+    [DecidableEq arity] [Fintype arity] [Hashable arity] {fsm : FSM arity} {n : Nat}
+  (circs : KInductionCircuits fsm n) where
+  hCInitCarryAssignCirc :
+    ∀ {env : Vars fsm.α arity 0 → Bool},
+      (circs.cInitCarryAssignCirc.eval env = false)
+      ↔ (∀ (s : fsm.α), fsm.initCarry s = env (Vars.state0 s))
+
+  hCSuccCarryAssignCirc :
+    ∀ {env : Vars fsm.α arity (n + 2) → Bool},
+      (circs.cSuccCarryAssignCirc.eval env = false)
+      ↔ (∀ (s : fsm.α) (i : Nat) (hi : i < n + 2),
+        env (Vars.stateN s (i + 1)) =
+          ((mkCarryAssignCircuitNAux fsm s i).map
+            (fun v => v.castLe (by omega))).eval env)
+  hCOutAssignCirc :
+    ∀ {env : Vars fsm.α arity (n + 2) → Bool},
+      (circs.cOutAssignCirc.eval env = false)
+      ↔ (∀ (i : Nat) (hi : i < n + 2),
+        (fsm.nextBitCirc none).eval
+          (fun x => match x with
+            | .inl s => env (Vars.stateN s i)
+            | .inr j => env (Vars.inputN j i)) =
+        env (Vars.outputs ⟨i, by omega⟩))
+  hCStatesUniqueCirc :
+    ∀ {env : Vars fsm.α arity (n) → Bool},
+      (circs.cStatesUniqueCirc.eval env = false)
+      ↔ (∀ (i j : Nat) (hij : i < j ∧ j ≤ n),
+        ∃ (s : fsm.α), env (Vars.stateN s i) ≠ env (Vars.stateN s j))
+
+attribute [simp] KInductionCircuits.IsLawful.hCInitCarryAssignCirc
+attribute [simp] KInductionCircuits.IsLawful.hCSuccCarryAssignCirc
+attribute [simp] KInductionCircuits.IsLawful.hCOutAssignCirc
+attribute [simp] KInductionCircuits.IsLawful.hCStatesUniqueCirc
 
 namespace KInductionCircuits
 
 variable {arity : Type _}
-  [DecidableEq arity] [Fintype arity] [Hashable arity]
   {fsm : FSM arity}
 
 /--
@@ -969,13 +1383,43 @@ def castCircLe {n m : Nat} (c : Circuit (Vars fsm.α arity n)) (hnm : n ≤ m :=
     Circuit (Vars fsm.α arity m) :=
   c.map (fun v => v.castLe hnm)
 
+@[simp]
+theorem eval_castCircLe_eq {n m : Nat} (c : Circuit (Vars fsm.α arity n))
+    (hnm : n ≤ m)
+    {env : Vars fsm.α arity m → Bool} :
+    (castCircLe c hnm).eval env = c.eval
+      (fun x => env (x.castLe hnm)) := by
+  simp [castCircLe, Circuit.eval_map]
+
+
+variable [DecidableEq arity] [Fintype arity] [Hashable arity]
+
 /-- Make the carry circuit for the k-induction circuits. -/
 def mkZero : KInductionCircuits fsm 0 where
   cInitCarryAssignCirc := mkInitCarryAssignCircuit fsm
   cSuccCarryAssignCirc := mkCarryAssignCircuitLeN fsm 1
   cOutAssignCirc := mkOutputAssignCircuitLeN fsm 1
-  cStatesUniqueCirc := mkAllPairsUniqueStatesCircuit fsm 1
+  cStatesUniqueCirc := mkAllPairsUniqueStatesCircuit fsm 0
 
+theorem IsLawful_mkZero {arity : Type _}
+    [DecidableEq arity] [Fintype arity] [Hashable arity]
+    (fsm : FSM arity) :
+    (mkZero (fsm := fsm)).IsLawful where
+  hCInitCarryAssignCirc := by
+    intro s
+    simp only [mkZero]
+    simp only [eval_mkInitCarryAssignCircuit_eq_false_iff]
+  hCSuccCarryAssignCirc := by
+    intro env
+    simp only [mkZero]
+    simp only [mkCarryAssignCircuitLeN_eq_false_iff]
+  hCOutAssignCirc := by
+    intro env
+    simp only [mkZero]
+    simp only [mkOutputAssignCircuitLeN_eq_false_iff]
+  hCStatesUniqueCirc := by
+    intro env
+    simp [mkZero, mkAllPairsUniqueStatesCircuit_eq_false_iff]
 
 -- NOTE [Circuit Equivalence As a quotient]:
 -- We ideally should have a notion of `Circuit.equiv`, which says that
@@ -998,10 +1442,95 @@ def mkSucc
       (mkOutputAssignCircuitN fsm (n + 2)) |||
       (castCircLe prev.cOutAssignCirc)
   , cStatesUniqueCirc :=
-      mkStateUniqueCircuitN fsm (n + 2) |||
+      mkStateUniqueCircuitN fsm (n + 1) |||
       (castCircLe prev.cStatesUniqueCirc)
   }
 
+theorem IsLawful_mkSucc_of_IsLawful {arity : Type _}
+    [DecidableEq arity] [Fintype arity] [Hashable arity]
+    {fsm : FSM arity} {n : Nat}
+    (prev : KInductionCircuits fsm n)
+    (hPrev : prev.IsLawful) :
+    (mkSucc prev).IsLawful where
+  hCInitCarryAssignCirc := by
+    simp only [mkSucc, castCircLe, Circuit.eval_map]
+    exact hPrev.hCInitCarryAssignCirc
+  hCSuccCarryAssignCirc := by
+    simp only [mkSucc, castCircLe, Circuit.eval_map]
+    simp [Circuit.eval_map]
+    intros env
+    constructor
+    · intros h s i hi
+      obtain ⟨h₁, h₂⟩ := h
+      rw [hPrev.hCSuccCarryAssignCirc] at h₂
+      by_cases hi : i < n + 2
+      · simp only [Vars.castLe_stateN_eq_stateN, Circuit.eval_map,
+        Vars.castLe_castLe_eq_castLe_self, mkCarryAssignCircuitNAux_eval_eq,
+        Vars.castLe_inputs_eq_inputs] at h₂
+        rw [h₂ s i hi]
+      · have hi : i = n + 2 := by omega
+        subst hi
+        apply h₁
+    · intros h
+      constructor
+      · intros s
+        simp only at h ⊢
+        rw [h s _ (by omega)]
+      · rw [hPrev.hCSuccCarryAssignCirc]
+        intros s i hi
+        simp only [Vars.castLe_stateN_eq_stateN, Circuit.eval_map,
+          Vars.castLe_castLe_eq_castLe_self, mkCarryAssignCircuitNAux_eval_eq,
+          Vars.castLe_inputs_eq_inputs] at h
+        simp only [Vars.castLe_stateN_eq_stateN, Circuit.eval_map,
+          Vars.castLe_castLe_eq_castLe_self, mkCarryAssignCircuitNAux_eval_eq,
+          Vars.castLe_inputs_eq_inputs]
+        rw [h s i (by omega)]
+
+  hCOutAssignCirc := by
+    simp only [mkSucc, castCircLe, Circuit.eval_map]
+    simp [Circuit.eval_map]
+    intros env
+    constructor
+    · intros h i hi
+      obtain ⟨h₁, h₂⟩ := h
+      rw [hPrev.hCOutAssignCirc] at h₂
+      by_cases hi : i < n + 2
+      · simp at h₁ h₂ ⊢
+        rw [h₂ i hi]
+      · have : i = n + 2 := by omega
+        subst this
+        apply h₁
+    · intros h
+      constructor
+      · simp only at h ⊢
+        rw [h]
+      · rw [hPrev.hCOutAssignCirc]
+        intros i hi
+        simp
+        apply h
+  hCStatesUniqueCirc := by
+    simp only [mkSucc, castCircLe, Circuit.eval_map]
+    simp [Circuit.eval_map]
+    intros env
+    constructor
+    · intros h i j hij
+      simp [mkStateUniqueCircuitN_eq_false_iff] at h
+      simp [hPrev.hCStatesUniqueCirc] at h
+      obtain ⟨h₁, h₂⟩ := h
+      by_cases hj : j ≤ n
+      · apply h₂ i j (by omega)
+      · have : j = n + 1 := by omega
+        subst this
+        apply h₁ i (by omega)
+    · intros h
+      constructor
+      · rw [mkStateUniqueCircuitN_eq_false_iff]
+        intros i hi
+        apply h (j := n + 1) (hij := by omega)
+      · simp [hPrev.hCStatesUniqueCirc]
+        intros i j hij
+        simp at h ⊢
+        apply h i j (by omega)
 /--
 The precondition that assigns all
 `s[n+1] = carry(s[n], i[n])` and assigns all `o[n+1] = out(s[n], i[n])`.
@@ -1010,6 +1539,137 @@ def mkSuccCarryAndOutsAssignPrecond (circs : KInductionCircuits fsm n) :
     Circuit (Vars fsm.α arity (n + 2)) :=
   circs.cOutAssignCirc |||
   circs.cSuccCarryAssignCirc
+
+/--
+Since the `mkSuccCarryAndOutsAssignPrecond` produces a large
+condition, we keep it as-is, and use it evaluating to false
+as a precondition.
+-/
+theorem eval_mkSuccCarryAndOutAssignPrecond_eq_false_iff₁
+  {circs : KInductionCircuits fsm n}
+  (hCircs : circs.IsLawful) :
+  ∀ (env : Vars fsm.α arity (n + 2) → Bool),
+  (mkSuccCarryAndOutsAssignPrecond circs).eval env = false ↔
+  (∀ (s : fsm.α) (i : Nat) (hi : i < n + 2),
+    env (Vars.stateN s (i + 1)) =
+      ((mkCarryAssignCircuitNAux fsm s i).map
+        (fun v => v.castLe (by omega))).eval env) ∧
+  (∀ (i : Nat) (hi : i < n + 2),
+    (fsm.nextBitCirc none).eval
+      (fun x => match x with
+        | .inl s => env (Vars.stateN s i)
+        | .inr j => env (Vars.inputN j i)) =
+    env (Vars.outputs ⟨i, by omega⟩)) := by
+  intro env
+  rw [mkSuccCarryAndOutsAssignPrecond]
+  simp only [Circuit.eval_or, Bool.or_eq_false_iff, hCircs, IsLawful.hCOutAssignCirc,
+    IsLawful.hCSuccCarryAssignCirc]
+  simp [Circuit.eval_map]
+  constructor
+  · intros h
+    obtain ⟨h₁, h₂⟩ := h
+    constructor
+    · intros s k hk
+      apply h₂ s k (by omega)
+    · intros k hk
+      apply h₁ k (by omega)
+  · intros h
+    obtain ⟨h₁, h₂⟩ := h
+    constructor
+    · intros k hk
+      apply h₂ k (by omega)
+    · intros s k hk
+      apply h₁ s k (by omega)
+
+
+@[simp]
+theorem mkSuccCarryAndOutsAssignPrecond_eval_eq_false_of_eq_envBool_of_envBitstream_of_state
+  {circs : KInductionCircuits fsm n}
+  (hCircs : circs.IsLawful)
+  (env : Vars fsm.α arity (n + 2) → Bool)
+  (s0 : fsm.α → Bool)
+  (hEnv : env = envBool_of_envBitstream_of_state fsm envBitstream s0 (n + 1)) :
+  (mkSuccCarryAndOutsAssignPrecond circs).eval env = false := by
+  rw [eval_mkSuccCarryAndOutAssignPrecond_eq_false_iff₁ hCircs env]
+  subst hEnv
+  simp [envBoolStart_of_envBitstream, envBool_of_envBitstream_of_state]
+  constructor
+  · intros s i hi
+    simp [Vars.stateN]
+    simp [Circuit.eval_map]
+    simp [envBoolStart_of_envBitstream, envBool_of_envBitstream_of_state,
+      Vars.stateN, Vars.inputN]
+    rw [FSM.carryWith, FSM.carry, FSM.nextBit]
+    simp
+    congr
+    ext x
+    rcases x with x | x
+    · rfl
+    · simp [Vars.inputN]
+  · intros i hi
+    congr
+    ext x
+    rcases x with x | x
+    · simp [Vars.stateN]
+      rfl
+    · simp [Vars.inputN]
+
+-- | TODO: remove duplication, reuse
+-- `mkSuccCarryAndOutsAssignPrecond_eval_eq_false_of_eq_envBool_of_envBitstream_of_state`
+-- to work.
+@[simp]
+theorem mkSuccCarryAndOutsAssignPrecond_eval_eq_false_of_eq_envBoolStart_of_envBitstream
+  {circs : KInductionCircuits fsm n}
+  (hCircs : circs.IsLawful)
+  (env : Vars fsm.α arity (n + 2) → Bool)
+  (hEnv : env = envBoolStart_of_envBitstream fsm envBitstream (n + 1)) :
+  (mkSuccCarryAndOutsAssignPrecond circs).eval env = false := by
+  rw [eval_mkSuccCarryAndOutAssignPrecond_eq_false_iff₁ hCircs env]
+  subst hEnv
+  simp [envBoolStart_of_envBitstream, envBool_of_envBitstream_of_state]
+  constructor
+  · intros s i hi
+    simp [Vars.stateN]
+    simp [Circuit.eval_map]
+    simp [envBoolStart_of_envBitstream, envBool_of_envBitstream_of_state,
+      Vars.stateN, Vars.inputN]
+    simp [FSM.carry, FSM.nextBit]
+    congr
+    ext x
+    rcases x with x | x
+    · simp
+    · simp
+  · intros i hi
+    simp [FSM.eval, FSM.nextBit]
+    congr
+    ext x
+    rcases x with x | x
+    · simp [Vars.stateN]
+    · simp [Vars.inputN]
+
+@[simp]
+theorem mkSuccCarryAndOutsAssignPrecond_eval_envBoolStart_of_envBitstream_eq_false
+  {circs : KInductionCircuits fsm n}
+  (hCircs : circs.IsLawful)
+  (envBitstream : _ ) :
+  (mkSuccCarryAndOutsAssignPrecond circs).eval
+    (envBoolStart_of_envBitstream fsm envBitstream (n + 1)) = false := by
+  apply mkSuccCarryAndOutsAssignPrecond_eval_eq_false_of_eq_envBoolStart_of_envBitstream <;>
+    solve
+    | assumption
+    | rfl
+
+@[simp]
+theorem mkSuccCarryAndOutsAssignPrecond_eval_envBool_of_envBitstream_of_state_eq_false
+  {circs : KInductionCircuits fsm n}
+  (hCircs : circs.IsLawful)
+  (envBitstream : _ ) :
+  (mkSuccCarryAndOutsAssignPrecond circs).eval
+    (envBool_of_envBitstream_of_state fsm envBitstream s0 (n + 1)) = false := by
+  apply mkSuccCarryAndOutsAssignPrecond_eval_eq_false_of_eq_envBool_of_envBitstream_of_state <;>
+    solve
+    | assumption
+    | rfl
 
 
 /--
@@ -1024,6 +1684,31 @@ def mkPostcondSafety (_circs : KInductionCircuits fsm n) :
     -- | then the output is fals for all i ≤ n.
     (mkOutEqZeroCircuitLeN fsm n)
 
+set_option linter.unusedVariables false in
+theorem eval_mkPostcondSafety_eq_false_iff
+    {circs : KInductionCircuits fsm n}
+    (hCircs : circs.IsLawful)
+    (env : Vars fsm.α arity (n + 1) → Bool) :
+    ((mkPostcondSafety circs).eval env = false) ↔
+    ((∀ (s : fsm.α), fsm.initCarry s = env ((Vars.state0 s))) →
+    (∀ (i : Nat) (hi : i < n + 1), env (Vars.outputs ⟨i, by omega⟩) = false)) := by
+  rw [mkPostcondSafety]
+  simp only [mkUnsatImpliesCircuit_eq_false_iff, Circuit.eval_map,
+    hCircs.hCInitCarryAssignCirc, IsLawful.hCOutAssignCirc]
+  simp
+  constructor
+  · intros h hinit i hi
+    simp only at h
+    rw [eval_mkInitCarryAssignCircuit_eq_false_iff] at h
+    rw [mkOutEqZeroCircuitLeN_eval_eq_false_iff] at h
+    apply h
+    apply hinit
+  · intros h
+    rw [mkOutEqZeroCircuitLeN_eval_eq_false_iff]
+    rw [eval_mkInitCarryAssignCircuit_eq_false_iff]
+    intros hpre
+    apply h
+    apply hpre
 /--
 The induction hypothesis circuit that checks that if
 the output is zero for all `i ≤ n`, then the output is zero at `i=n+1`.
@@ -1036,6 +1721,22 @@ def mkPostcondIndHypNoCycleBreaking {n} (_circs : KInductionCircuits fsm n) :
     -- | Then the output is zero at `i = n+1`
     (mkOutEqZeroCircuitN fsm <| n+1)
 
+set_option linter.unusedVariables false in
+theorem mkPostcondIndHypNoCycleBreaking_eq_false_iff
+    {circs : KInductionCircuits fsm n}
+    (hCircs : circs.IsLawful)
+    (env : Vars fsm.α arity (n + 2) → Bool) :
+    ((mkPostcondIndHypNoCycleBreaking circs).eval env = false) ↔
+    ((∀ (i : Nat) (hi : i < n + 1), env (Vars.outputs ⟨i, by omega⟩) = false) →
+    env (Vars.outputs ⟨n + 1, by omega⟩) = false) := by
+  rw [mkPostcondIndHypNoCycleBreaking]
+  simp only [mkUnsatImpliesCircuit_eq_false_iff, Circuit.eval_map,
+    hCircs.hCOutAssignCirc]
+  simp
+  constructor
+  · simp [mkOutEqZeroCircuitLeN_eval_eq_false_iff]
+  · simp [mkOutEqZeroCircuitLeN_eval_eq_false_iff]
+
 /--
 If the initial state `s[0] = initCarry`,
 and `states[i+1] = carry(states[i], inputs[i])` and `out[i] = out(states[i], inputs[i])`,
@@ -1046,6 +1747,60 @@ def mkSafetyCircuit (circs : KInductionCircuits fsm n) :
   mkUnsatImpliesCircuit
     (mkSuccCarryAndOutsAssignPrecond circs)
     (castCircLe <| mkPostcondSafety circs)
+
+theorem mkSafetyCircuit_eval_eq_false_iff₁
+    {circs : KInductionCircuits fsm n}
+    (hCircs : circs.IsLawful)
+    (env : Vars fsm.α arity (n + 2) → Bool) :
+    ((mkSafetyCircuit circs).eval env = false) ↔
+    ((mkSuccCarryAndOutsAssignPrecond circs).eval env = false →
+      (∀ (s : fsm.α), fsm.initCarry s = env (Vars.state0 s)) →
+      (∀ (i : Nat) (hi : i < n + 1), env (Vars.outputs ⟨i, by omega⟩) = false)) := by
+  rw [mkSafetyCircuit]
+  simp only [mkUnsatImpliesCircuit_eq_false_iff, Circuit.eval_map,
+    hCircs.hCInitCarryAssignCirc, hCircs.hCOutAssignCirc]
+  simp
+  constructor
+  · intros h hinit hsafe i hi
+    rw [eval_mkPostcondSafety_eq_false_iff] at h
+    · simp at h
+      apply h
+      · apply hinit
+      · apply hsafe
+      · omega
+    · apply hCircs
+  · intros h
+    intros hPrecond
+    rw [eval_mkPostcondSafety_eq_false_iff]
+    simp
+    apply h
+    · apply hPrecond
+    · apply hCircs
+
+/--
+Safe upto n steps, given that `mkSafetyCircuit.eval env = false` for all `env`.
+-/
+theorem mkSafetyCircuit_eval_eq_false_thm
+    {circs : KInductionCircuits fsm n}
+    (hCircs : circs.IsLawful)
+    (h : ∀ (env : _), (mkSafetyCircuit circs).eval env = false) :
+    (∀ (envBitstream : _) (i : Nat), i < n + 1 → fsm.eval envBitstream i = false) := by
+  intros envBitstream i hi
+  let env := envBoolStart_of_envBitstream fsm envBitstream (n + 1)
+  specialize h env
+  rw [mkSafetyCircuit_eval_eq_false_iff₁ hCircs env] at h
+  subst env
+  have := mkSuccCarryAndOutsAssignPrecond_eval_envBoolStart_of_envBitstream_eq_false
+    hCircs envBitstream
+  specialize h this
+  clear this
+  simp at h
+  specialize h ?precond
+  · intros s
+    simp [envBoolStart_of_envBitstream, envBool_of_envBitstream_of_state, Vars.stateN]
+  · simp [envBoolStart_of_envBitstream, envBool_of_envBitstream_of_state, Vars.outputs] at h
+    apply h
+    · omega
 
 /--
 If states[i+1] = carry(states[i], inputs[i]) and
@@ -1059,6 +1814,14 @@ def mkIndHypCircuitNoCycleBreaking (circs : KInductionCircuits fsm n) :
     (mkSuccCarryAndOutsAssignPrecond circs)
     -- | Then the output is zero at `i = n+1`
     (mkPostcondIndHypNoCycleBreaking circs)
+
+@[simp]
+theorem mkIndHypCircuitNoCycleBreaking_eval_eq_false_iff
+    {circs : KInductionCircuits fsm n}
+    (env : Vars fsm.α arity (n + 2) → Bool) :
+    ((mkIndHypCircuitNoCycleBreaking circs).eval env = false) ↔
+    ((mkSuccCarryAndOutsAssignPrecond circs).eval env = false → (mkPostcondIndHypNoCycleBreaking circs).eval env = false) := by
+  simp [mkIndHypCircuitNoCycleBreaking]
 
 /--
 If states[i+1] = carry(states[i], inputs[i]) and
@@ -1075,6 +1838,501 @@ def mkIndHypCycleBreaking (circs : KInductionCircuits fsm n) :
       -- | Then the output is zero at `i = n+1`
       (mkPostcondIndHypNoCycleBreaking circs))
 
+theorem mkIndHypCycleBreaking_eval_eq_false_iff₁
+    {circs : KInductionCircuits fsm n}
+    (env : Vars fsm.α arity (n + 2) → Bool) :
+    ((mkIndHypCycleBreaking circs).eval env = false) ↔
+    ((mkSuccCarryAndOutsAssignPrecond circs).eval env = false →
+      (circs.cStatesUniqueCirc.eval (fun x => env (x.castLe (by omega))) = false) →
+      (mkPostcondIndHypNoCycleBreaking circs).eval env = false) := by
+  simp [mkIndHypCycleBreaking, mkUnsatImpliesCircuit_eq_false_iff, Circuit.eval_map]
+
+
+/--
+the states in `fsm` starting from state `s0`, with inputs `inputs` is all unique.
+-/
+def StatesUniqueLe (fsm : FSM arity) (s0 : fsm.α → Bool) (inputs : arity → BitStream) (n : Nat) : Prop :=
+  ∀ (i j : Nat), i < j ∧ j ≤ n → (fsm.carryWith s0 inputs i) ≠ (fsm.carryWith s0 inputs j)
+
+@[simp] theorem StatesUniqueLe_zero {fsm : FSM arity} {s0 : fsm.α → Bool} {inputs : arity → BitStream} :
+  StatesUniqueLe fsm s0 inputs 0 := by
+  intros i j hij
+  simp at hij
+  omega
+
+/--
+Show what the induction hypothesis with cycle breaking circuit implies.
+-/
+theorem  mkIndHypCycleBreaking_eval_eq_false_thm_aux
+  {circs : KInductionCircuits fsm n}
+  (hcircs : circs.IsLawful)
+  (h : ∀ (env : _), (mkIndHypCycleBreaking circs).eval env = false) :
+  (∀ (envBitstream : _) (s0 : _), (∀ (i : Nat) (j : Nat), i < j ∧ j ≤ n →
+      (fsm.carryWith s0 envBitstream i) ≠ (fsm.carryWith s0 envBitstream j)) →
+      (∀ (k : Nat), k < n + 1 → fsm.evalWith s0 envBitstream k = false) →
+      (fsm.evalWith s0 envBitstream (n + 1) = false)) := by
+  simp [mkIndHypCycleBreaking_eval_eq_false_iff₁] at h
+  intros envBitstream s0 huniq hind
+  let env := envBool_of_envBitstream_of_state fsm envBitstream s0 (n + 1)
+  specialize h env
+  specialize h ?precond ?huniq
+  · apply mkSuccCarryAndOutsAssignPrecond_eval_eq_false_of_eq_envBool_of_envBitstream_of_state
+      (envBitstream := envBitstream) (s0 := s0)
+    · exact hcircs
+    · simp [env]
+  · rw [hcircs.hCStatesUniqueCirc]
+    intros i j hij
+    specialize huniq i j hij
+    -- show that `(Vars.stateN s i)` equals `fsm.eval ...`
+    -- | TODO: cleanup this, with
+    -- envBoolStart_of_envBitstream,
+    -- envBool_of_envBitstream_of_state, Vars.stateN
+    -- as a single lemma.
+    simp [env, envBoolStart_of_envBitstream, envBool_of_envBitstream_of_state, Vars.stateN]
+    rw [← Function.ne_iff]
+    exact huniq
+    -- specialize huniq i j hij
+  · rw [mkPostcondIndHypNoCycleBreaking_eq_false_iff] at h
+    simp [env, envBoolStart_of_envBitstream, envBool_of_envBitstream_of_state] at h
+    apply h
+    apply hind
+    exact hcircs
+
+
+/-- Show that the 'mkIndHypCycleBreaking' theorem establishes safety for all unique paths. -/
+theorem  mkIndHypCycleBreaking_eval_eq_false_thm
+  {circs : KInductionCircuits fsm n}
+  (hcircs : circs.IsLawful)
+  (h : ∀ (env : _), (mkIndHypCycleBreaking circs).eval env = false) :
+  (∀ (envBitstream : _) (s0 : _), StatesUniqueLe fsm s0 envBitstream n →
+      (∀ (k : Nat), k < n + 1 → fsm.evalWith s0 envBitstream k = false) →
+      (fsm.evalWith s0 envBitstream (n + 1) = false)) := by
+  simp [StatesUniqueLe]
+  intros envBitstream s0 hind
+  apply mkIndHypCycleBreaking_eval_eq_false_thm_aux (circs := circs) (hcircs := hcircs)
+  · apply h
+  · intros i j hij
+    apply hind
+    · omega
+    · omega
+
+
+/-- induction principle with a uniform bound 'bound' in place. -/
+@[elab_as_elim]
+theorem ind_principle₂  {motive : Nat → Prop} (bound : Nat)
+  (hBase : ∀ i ≤ bound, motive i)
+  (hInd : ∀ (i : Nat),
+    bound < i →
+    ((∀ (k : Nat), k < bound → motive (i - k - 1)) → motive i)) :
+  ∀ k, motive k := by
+  intros k
+  induction k using Nat.strong_induction_on
+  case h k ihk =>
+    by_cases hK : k ≤ bound
+    · apply hBase
+      omega
+    · have : ∃ δ, k = δ + (bound) := by exists (k - (bound)); omega
+      obtain ⟨δ, hδ⟩ := this
+      subst hδ
+      apply hInd
+      omega
+      intros ε  hε
+      apply ihk
+      omega
+
+
+/--
+`eval` is false iff we establish the safety and induction hypothesis.
+-/
+theorem eval_eq_false_of_eval_eq_false_le_n_of_eval_eq_false_le_n_of_eval_eq_false_le_n {n : Nat}
+    {arity : Type _} [DecidableEq arity] [Fintype arity] [Hashable arity]
+    (p : FSM arity)
+    (hs : ∀ (envBitstream : arity → BitStream), ∀ i ≤ n, p.eval envBitstream i = false)
+    (hind : ∀ (state : p.α → Bool) (envBitstream : arity → BitStream),
+    (∀ i ≤ n, p.evalWith state envBitstream i = false) →
+      p.evalWith state envBitstream (n + 1) = false)
+    :
+    ∀ (envBitstream : arity → BitStream) (i : Nat), p.eval envBitstream i = false := by
+  intros envBitstream i
+  rw [FSM.eval_eq_evalWith_initCarry]
+  induction i using Nat.strong_induction_on
+  case h i hStrongI =>
+    induction i using ind_principle₂ n
+    case hBase i hi =>
+      apply hs
+      omega
+    case hInd j hjLt hjInd =>
+      rw [show j = (j - (n + 1)) + (n + 1) by omega]
+      rw [FSM.evalWith_add_eq_evalWith_carryWith]
+      apply hind
+      · intros i hi
+        rw [← FSM.evalWith_add_eq_evalWith_carryWith]
+        rw [show j - (n + 1)  + i = j - (n + 1 - i) by omega]
+        rw [show j - (n + 1 - i) = j - ((n - i)) - 1 by omega]
+        by_cases hi : i = 0
+        · subst hi
+          simp
+          apply hStrongI
+          omega
+        · apply hjInd
+          · omega
+          · intros k hk; apply hStrongI; omega
+
+/--
+Make a simple path corresponding to inputs[:n],
+such that carryWith fsm s0 inputs n = carryWith fsm s0 out.inputs out.k,
+where `k ≤ n`, and moreover, `out.inputs` is a simple path.
+-/
+structure SimplePathOfPath (fsm : FSM arity) (s0 : fsm.α → Bool) (n : Nat) (inputs : arity → BitStream) where
+  simplePath : arity → BitStream
+  k : Nat
+  hkLt : k ≤ n
+  hCarryWith :  fsm.carryWith s0 inputs n = fsm.carryWith s0 simplePath k
+  /-- We pick a subsequence of paths. -/
+  hCarryWith_of_le : ∀ (i : Nat), i ≤ k →
+    ∃ j : Nat, j ≤ n ∧ fsm.carryWith s0 simplePath i = fsm.carryWith s0 inputs j
+  hStatesUniqueLe : StatesUniqueLe fsm s0 simplePath k
+
+
+/--
+This shows that `fsm.carry` at the end is unchanged.
+-/
+def SimplePathOfPath.hCarry (this : SimplePathOfPath fsm s0 n inputs)
+  (hs0 : s0 = fsm.initCarry := by rfl) :
+    fsm.carry inputs n = fsm.carry this.simplePath this.k := by
+  rw [FSM.carry_eq_carryWith_initCarry]
+  subst hs0
+  apply this.hCarryWith
+
+/--
+Find the occurrence of a state 's' in the simple path.
+-/
+noncomputable def SimplePathOfPath.findState?
+  (_this : SimplePathOfPath fsm s0 n inputs)
+  (s : fsm.α → Bool) :
+    { k? : Option Nat // ∀ (k : Nat), k? = some k ↔ k ≤ n ∧ fsm.carryWith s0 inputs k = s ∧ ∀ l < k, fsm.carryWith s0 inputs l ≠ s } :=
+  let states :=
+    (List.range (n + 1)).map fun i =>
+      fsm.carryWith s0 inputs i
+  let out := states.findIdx? (fun t => t = s)
+  match hout : out with
+  | none =>
+    ⟨none, by
+      simp only [reduceCtorEq, ne_eq, false_iff, not_and, not_forall, Classical.not_imp,
+        Decidable.not_not]
+      subst out
+      have := List.findIdx?_eq_none_iff |>.mp hout
+      subst states
+      simp only [List.mem_map, List.mem_range, decide_eq_false_iff_not, forall_exists_index,
+        and_imp, forall_apply_eq_imp_iff₂] at this
+      intros k hk
+      intros hcontra
+      specialize this k (by omega)
+      contradiction
+    ⟩
+  | some idx =>
+    ⟨some idx, by
+      have := List.findIdx?_eq_some_iff_findIdx_eq .. |>.mp hout
+      obtain ⟨h₁, h₂⟩ := this
+      intros k
+      simp only [Option.some.injEq, ne_eq]
+      constructor
+      · intros hk
+        subst hk
+        constructor
+        · simp only [List.findIdx?_map, List.length_map, List.length_range, out, states] at *
+          omega
+        · have := List.findIdx_eq h₁ |>.mp h₂
+          simp at this
+          obtain ⟨hidx, hfirst⟩ := this
+          simp only [List.getElem_map, List.getElem_range, states] at hidx
+          constructor
+          · simp only [hidx]
+          · intros l hl
+            simp only [List.getElem_map, List.getElem_range, states] at hfirst
+            apply hfirst
+            omega
+      . intros hk
+        obtain ⟨hkLt, hk, hneq⟩ := hk
+        rw [← h₂]
+        have hkLt₂ : k < states.length := by
+          simp only [List.length_map, List.length_range, states]
+          omega
+        apply (List.findIdx_eq hkLt₂ |>.mpr)
+        simp only [List.getElem_map, List.getElem_range, hk, decide_true, decide_eq_false_iff_not,
+          true_and, states]
+        apply hneq
+    ⟩
+
+
+
+
+/--
+set values for index `i` in the environment `x`,
+where `v` is the value to set.
+-/
+def envBitstream_set (x : arity → BitStream) (n : Nat) (v : arity → Bool) :
+    arity → BitStream :=
+  fun a j => if j = n then v a else x a j
+
+@[simp]
+def envBitstream_set_self_eq_self (x : arity → BitStream) (n : Nat) (v : arity → Bool) :
+    (envBitstream_set x n (fun a => x a n)) = x := by
+  ext a i
+  simp [envBitstream_set]
+  intros hi
+  subst hi
+  rfl
+
+@[simp]
+theorem envBitstream_set_eq_self_of_ne {x : arity → BitStream}
+    {n k : Nat} {v : arity → Bool} {a : arity} (hneq : k ≠ n) :
+  (envBitstream_set x n v) a k = x a k := by
+  simp [envBitstream_set, hneq]
+
+@[simp]
+theorem envBitstream_set_eq_of_eq {x : arity → BitStream} {n k : Nat} {v : arity → Bool}
+    {a : arity} (hneq : k = n) :
+    (envBitstream_set x n v) a k = v a := by
+  simp [envBitstream_set, hneq]
+
+@[simp]
+theorem envBitstream_set_eq_of_eq₂   {x : arity → BitStream}
+    {n : Nat} {v : arity → Bool} {a : arity} :
+  (envBitstream_set x n v) a n = v a := by
+  simp [envBitstream_set]
+
+
+/--
+There always exists a simple path of a given path,
+which is shorter than the path, and ends at the same state.
+Luckily, we don't care about this being executable or fast.
+To ensure that we do not use the performance of this procedure,
+we mark it `noncomputable`.
+-/
+axiom mkSimplePathOfPath (fsm : FSM arity)
+    (s0 : fsm.α → Bool) (n : Nat) (inputs : arity → BitStream) :
+    SimplePathOfPath fsm s0 n inputs
+/-
+  :=
+  match hn : n with
+  | 0 => {
+    simplePath := inputs,
+    k := 0,
+    hkLt := by omega,
+    hCarryWith := rfl,
+    hStatesUniqueLe := StatesUniqueLe_zero,
+    hCarryWith_of_le := by
+      intros i hi
+      simp [hi]
+      have : i = 0 := by omega
+      subst this
+      simp
+  }
+  | n' + 1 =>
+    let path' := mkSimplePathOfPath fsm s0 n' inputs
+    let sn := fsm.carryWith s0 inputs n
+    match path'.findState? sn with
+    | ⟨none, hnone⟩ => {
+      simplePath := envBitstream_set path'.simplePath n (fun a => inputs a n),
+      k := path'.k + 1,
+      hkLt := by
+        have := path'.hkLt
+        omega,
+      hCarryWith := by
+        have := path'.hCarryWith
+        sorry
+
+      hCarryWith_of_le := by
+        sorry
+      hStatesUniqueLe := by
+        have := path'.hStatesUniqueLe
+        simp [StatesUniqueLe] at this ⊢
+        have hklt := path'.hkLt
+        intros i j hi hj
+        by_cases hj : j = path'.k + 1
+        · sorry
+        · have hEnvI : fsm.carryWith s0 (envBitstream_set path'.simplePath n (fun a => inputs a n)) i =
+              fsm.carryWith s0 path'.simplePath i := by
+            apply FSM.carryWith_congrEnv
+            intros a k hk
+            rw [envBitstream_set_eq_self_of_ne]
+            omega
+          have hEnvJ : fsm.carryWith s0 (envBitstream_set path'.simplePath n (fun a => inputs a n)) j =
+              fsm.carryWith s0 path'.simplePath j := by
+            apply FSM.carryWith_congrEnv
+            intros a k hk
+            rw [envBitstream_set_eq_self_of_ne]
+            omega
+          rw [hEnvI, hEnvJ]
+          apply this
+          · omega
+          · omega
+    }
+    | ⟨some k, hsome⟩ => sorry
+-/
+
+/-- Safety on all simple paths implies safety on all paths. -/
+theorem evalWith_eq_false_of_evalWith_eq_false_of_StatesUniqueLe (fsm : FSM arity)
+    (h : ∀ (inputs : _) (n : Nat),
+      StatesUniqueLe fsm fsm.initCarry inputs n →
+      fsm.evalWith fsm.initCarry inputs n = false)
+    (n : Nat) (inputs : _) :
+  fsm.evalWith fsm.initCarry inputs n = false := by
+  have := mkSimplePathOfPath fsm fsm.initCarry n inputs
+  simp [FSM.evalWith_eq_outputWith_carryWith]
+  rw [FSM.carry_eq_carryWith_initCarry]
+  rw [this.hCarryWith]
+  simp [FSM.evalWith_eq_outputWith_carryWith] at h
+  -- | make an 'env' that uses the input at 'k' to get the output.
+  let env' := fun a i => if i = this.k then inputs a n else this.simplePath a i
+  have hInputs : (fun a => inputs a n) = (fun a => env' a this.k) := by
+    simp [env']
+  rw [hInputs]
+  rw [FSM.carryWith_congrEnv (y := env')]
+  · rw [← FSM.evalWith_eq_outputWith_carryWith]
+    apply h
+    -- | TODO: need lemmas here.
+    simp [StatesUniqueLe]
+    intros i j hi hj
+    have hUnique := this.hStatesUniqueLe
+    simp [StatesUniqueLe] at hUnique
+    specialize hUnique i j (by omega) (by omega)
+    have hEnvI : fsm.carry env' i = fsm.carry this.simplePath i := by
+      apply FSM.carry_congrEnv
+      intros a l hl
+      simp [env', hl, show l ≠ this.k by omega]
+    have hEnvJ : fsm.carry env' j = fsm.carry this.simplePath j := by
+      apply FSM.carry_congrEnv
+      intros a l hl
+      simp [env', hl, show l ≠ this.k by omega]
+    rw [hEnvI, hEnvJ]
+    apply hUnique
+  · intros a k hk
+    simp [env']
+    intros hk'
+    omega
+
+
+/--
+Evaluating at the created simple path equals evaluating at the original path.
+-/
+def SimplePathOfPath.hEvalWith (this : SimplePathOfPath fsm s0 (K + 1) env) :
+    fsm.evalWith s0 env (K + 1) =
+    fsm.evalWith s0
+      (envBitstream_set this.simplePath (this.k) (fun a => env a (K + 1))) this.k := by
+  rw [FSM.evalWith_eq_outputWith_carryWith]
+  rw [FSM.evalWith_eq_outputWith_carryWith]
+  rw [this.hCarryWith]
+  rw [FSM.carryWith_congrEnv (y := envBitstream_set this.simplePath (this.k) (fun a => env a (K + 1)))]
+  · congr
+    ext i
+    simp
+  · intros a i hi
+    rw [envBitstream_set_eq_self_of_ne (by omega)]
+
+/--
+If we have all unique states upto `K`, then we have unique states upto
+`k' \leq K` on an `env'`, as long as `env` and `env'` match upto the required length.
+-/
+theorem StatesUniqueLe_of_StatesUniqueLe_congr
+  {K k' : Nat}
+  {fsm : FSM arity} {s0 : fsm.α → Bool}
+  {env env' : arity → BitStream}
+  {this : StatesUniqueLe fsm s0 env K}
+  (hk' : k' ≤ K)
+  (henv' : ∀ (a : arity) (i : Nat), i ≤ k' → env' a i = env a i) :
+  StatesUniqueLe fsm s0 env' k' := by
+  simp [StatesUniqueLe] at ⊢ this
+  intros i j hii hj
+  have hEnvI : fsm.carryWith s0 env' i = fsm.carryWith s0 env i := by
+    apply FSM.carryWith_congrEnv
+    intros a l hl
+    apply henv'
+    omega
+  have hEnvJ : fsm.carryWith s0 env' j = fsm.carryWith s0 env j := by
+    apply FSM.carryWith_congrEnv
+    intros a l hl
+    apply henv'
+    omega
+  rw [hEnvI, hEnvJ]
+  apply this
+  · omega
+  · omega
+
+/-- Safety for all simple paths. -/
+axiom all_simple_paths_good
+    (fsm : FSM arity) (K : Nat)
+    (hsafety : ∀ (i : Nat) (env : _) , i < K + 1 → fsm.evalWith fsm.initCarry env i = false)
+    (hind : ∀ (s0 : _) (env : _),
+       StatesUniqueLe fsm s0 env K →
+       (∀ (i : Nat), i ≤ K  → fsm.evalWith s0 env i = false) →
+        fsm.evalWith s0 env (K + 1) = false) :
+  ∀ (env : _) (n : Nat),
+    StatesUniqueLe fsm fsm.initCarry env n →
+    fsm.evalWith fsm.initCarry env n = false
+  -- := by sorry
+
+/--
+info: 'ReflectVerif.BvDecide.KInductionCircuits.all_simple_paths_good' depends on axioms: [ReflectVerif.BvDecide.KInductionCircuits.all_simple_paths_good]
+-/
+#guard_msgs in #print axioms all_simple_paths_good
+
+/--
+Safety for all paths, given that kinduction base case holds,
+and that we can apply k-induction to simple paths.
+-/
+theorem all_paths_good_of_kbase_of_simple_path_kind
+    (fsm : FSM arity) (K : Nat)
+    (hsafety : ∀ (i : Nat) (env : _),
+      i < K + 1 → fsm.evalWith fsm.initCarry env i = false)
+    (hind : ∀ (s0 : _) (env : _),
+      StatesUniqueLe fsm s0 env K →
+      (∀ (i : Nat), i ≤ K → fsm.evalWith s0 env i = false) →
+      fsm.evalWith s0 env (K + 1) = false) :
+  ∀ (env : _) (n : Nat),
+    fsm.evalWith fsm.initCarry env n = false := by
+  intros env n
+  apply evalWith_eq_false_of_evalWith_eq_false_of_StatesUniqueLe
+  apply all_simple_paths_good (K := K)
+  · apply hsafety
+  · intros s0 env hUnique hindPrecond
+    apply hind
+    · apply hUnique
+    · apply hindPrecond
+
+/--
+Safety on all paths, given that our evaluation of
+`mkSafetyCircuit` is false, and `mkIndHypCycleBreaking` is false.
+This is the theorem that is hooked to the external world.
+-/
+theorem eval_eq_false_of_mkIndHypCycleBreaking_eval_eq_false_of_mkSafetyCircuit_eval_eq_false
+    {circs : KInductionCircuits fsm K}
+    (hCircs : circs.IsLawful)
+    (hSafety : ∀ (env : _), (mkSafetyCircuit circs).eval env = false)
+    (hIndHyp : ∀ (env : _), (mkIndHypCycleBreaking circs).eval env = false) :
+    (∀ (envBitstream : _), fsm.eval envBitstream i = false) := by
+  intros envBitstream
+  obtain hSafety := mkSafetyCircuit_eval_eq_false_thm hCircs hSafety
+  obtain hIndHyp := mkIndHypCycleBreaking_eval_eq_false_thm hCircs hIndHyp
+  apply all_paths_good_of_kbase_of_simple_path_kind (K :=  K)
+  · intros k env hk
+    apply hSafety
+    omega
+  · intros s0 env hUnique hind
+    apply hIndHyp
+    · apply hUnique
+    · intros i hi
+      apply hind
+      omega
+/--
+info: 'ReflectVerif.BvDecide.KInductionCircuits.eval_eq_false_of_mkIndHypCycleBreaking_eval_eq_false_of_mkSafetyCircuit_eval_eq_false' depends on axioms: [propext,
+ Classical.choice,
+ Quot.sound,
+ ReflectVerif.BvDecide.KInductionCircuits.all_simple_paths_good,
+ ReflectVerif.BvDecide.KInductionCircuits.mkSimplePathOfPath]
+-/
+#guard_msgs in #print axioms eval_eq_false_of_mkIndHypCycleBreaking_eval_eq_false_of_mkSafetyCircuit_eval_eq_false
 
 def stats {arity : Type _}
     [DecidableEq arity] [Fintype arity] [Hashable arity]
